More work in improving organization.

MinimunLogic/LogicBase.v
@@ -15,34 +15,47 @@ Class ProofTheory (L: Language): Type := {
   derivable: context -> expr -> Prop
 }.
 
-Class Semantics (L: Language): Type := {
-  model: Type;
+Class Model: Type := {
+  model: Type
+}.
+
+Class Semantics (L: Language) (MD: Model): Type := {
   satisfies: model -> expr -> Prop
+}.
+
+Class NormalLanguage (L: Language): Type := {
+  impp: expr -> expr -> expr
+}.
+
+Class KripkeModel (MD: Model): Type := {
+  Kmodel: Type;
+  Kworlds: Kmodel -> Type;
+  build_model: forall M: Kmodel, Kworlds M -> model
 }.
 
 Definition consistent {L: Language} {Gamma: ProofTheory L}: context -> Prop :=
   fun Phi =>
     exists x: expr, ~ derivable Phi x.
 
-Definition consequence {L: Language} {SM: Semantics L}: context -> expr -> Prop :=
+Definition consequence {L: Language} {MD: Model} {MD: Model} {SM: Semantics L MD}: context -> expr -> Prop :=
   fun Phi y =>
     forall m: model, (forall x, Phi x -> satisfies m x) -> satisfies m y.
 
-Definition valid {L: Language} {SM: Semantics L}: expr -> Prop :=
+Definition valid {L: Language} {MD: Model} {SM: Semantics L MD}: expr -> Prop :=
   fun x =>
     forall m: model, satisfies m x.
 
-Definition satisfiable {L: Language} {SM: Semantics L}: context -> Prop :=
+Definition satisfiable {L: Language} {MD: Model} {SM: Semantics L MD}: context -> Prop :=
   fun Phi =>
     exists m: model, forall x: expr, Phi x -> satisfies m x.
 
-Definition sound {L: Language} (Gamma: ProofTheory L) (SM: Semantics L): Prop :=
+Definition sound {L: Language} (Gamma: ProofTheory L) {MD: Model} (SM: Semantics L MD): Prop :=
   forall x: expr, provable x -> valid x.
 
-Definition weakly_complete {L: Language} (Gamma: ProofTheory L) (SM: Semantics L): Prop :=
+Definition weakly_complete {L: Language} (Gamma: ProofTheory L) {MD: Model} (SM: Semantics L MD): Prop :=
   forall x: expr, valid x -> provable x.
 
-Definition strongly_complete {L: Language} (Gamma: ProofTheory L) (SM: Semantics L): Prop :=
+Definition strongly_complete {L: Language} (Gamma: ProofTheory L) {MD: Model} (SM: Semantics L MD): Prop :=
   forall (Phi: context) (x: expr), consequence Phi x -> derivable Phi x.
 
 Notation "m  |=  x" := (satisfies m x) (at level 70, no associativity) : logic_base.
@@ -50,5 +63,8 @@ Notation "|==  x" := (valid x) (at level 71, no associativity) : logic_base.
 Notation "Phi  |==  x" := (consequence Phi x) (at level 70, no associativity) : logic_base.
 Notation "|--  x" := (provable x) (at level 71, no associativity) : logic_base.
 Notation "Phi  |--  x" := (derivable Phi x) (at level 70, no associativity) : logic_base.
+Notation "'KRIPKE:'  M , m" := (build_model M m) (at level 59, no associativity) : logic_base.
+Notation "x --> y" := (impp x y) (at level 55, right associativity) : logic_base.
+
 
 
