MinimunLogic/MinimunLogic.v
@@ -6,12 +6,6 @@ Local Open Scope logic_base.
 
 (* TODO: split language from logic. *)
 
-Class NormalLanguage (L: Language): Type := {
-  impp: expr -> expr -> expr
-}.
-
-Notation "x --> y" := (impp x y) (at level 55, right associativity) : logic_base.
-
 Definition multi_imp {L: Language} {nL: NormalLanguage L} (xs: list expr) (y: expr): expr :=
   fold_right impp y xs.
 
