PropositionalLogic/Sound_Classical_Trivial.v
@@ -11,7 +11,7 @@ Local Open Scope PropositionalLogic.
 
 Lemma sound_modus_ponens {Var: Type}:
   forall x y: @expr (PropositionalLanguage.L Var),
-    forall m: @model _ (TrivialSemantics.SM Var),
+    forall m: @model (TrivialSemantics.MD Var),
       m |= (x --> y) -> m |= x -> m |= y.
 Proof.
   intros.
@@ -20,7 +20,7 @@ Qed.
 
 Lemma sound_axiom1 {Var: Type}:
   forall x y: @expr (PropositionalLanguage.L Var),
-    forall m: @model _ (TrivialSemantics.SM Var),
+    forall m: @model (TrivialSemantics.MD Var),
       m |= x --> y --> x.
 Proof.
   intros; intros ? ?; auto.
@@ -28,7 +28,7 @@ Qed.
 
 Lemma sound_axiom2 {Var: Type}:
   forall x y z: @expr (PropositionalLanguage.L Var),
-    forall m: @model _ (TrivialSemantics.SM Var),
+    forall m: @model (TrivialSemantics.MD Var),
       m |= (x --> y --> z) --> (x --> y) --> (x --> z).
 Proof.
   intros.
@@ -41,7 +41,7 @@ Qed.
 
 Lemma sound_andp_intros {Var: Type}:
   forall x y: @expr (PropositionalLanguage.L Var),
-    forall m: @model _ (TrivialSemantics.SM Var),
+    forall m: @model (TrivialSemantics.MD Var),
       m |= x --> y --> x && y.
 Proof.
   intros.
@@ -52,7 +52,7 @@ Qed.
 
 Lemma sound_andp_elim1 {Var: Type}:
   forall x y: @expr (PropositionalLanguage.L Var),
-    forall m: @model _ (TrivialSemantics.SM Var),
+    forall m: @model (TrivialSemantics.MD Var),
       m |= x && y --> x.
 Proof.
   intros.
@@ -62,7 +62,7 @@ Qed.
 
 Lemma sound_andp_elim2 {Var: Type}:
   forall x y: @expr (PropositionalLanguage.L Var),
-    forall m: @model _ (TrivialSemantics.SM Var),
+    forall m: @model (TrivialSemantics.MD Var),
       m |= x && y --> y.
 Proof.
   intros.
@@ -72,7 +72,7 @@ Qed.
 
 Lemma sound_orp_intros1 {Var: Type}:
   forall x y: @expr (PropositionalLanguage.L Var),
-    forall m: @model _ (TrivialSemantics.SM Var),
+    forall m: @model (TrivialSemantics.MD Var),
       m |= x --> x || y.
 Proof.
   intros.
@@ -83,7 +83,7 @@ Qed.
 
 Lemma sound_orp_intros2 {Var: Type}:
   forall x y: @expr (PropositionalLanguage.L Var),
-    forall m: @model _ (TrivialSemantics.SM Var),
+    forall m: @model (TrivialSemantics.MD Var),
       m |= y --> x || y.
 Proof.
   intros.
@@ -94,7 +94,7 @@ Qed.
 
 Lemma sound_orp_elim {Var: Type}:
   forall x y z: @expr (PropositionalLanguage.L Var),
-    forall m: @model _ (TrivialSemantics.SM Var),
+    forall m: @model (TrivialSemantics.MD Var),
       m |= (x --> z) --> (y --> z) --> (x || y --> z).
 Proof.
   intros.
@@ -105,7 +105,7 @@ Qed.
 
 Lemma sound_falsep_elim {Var: Type}:
   forall x: @expr (PropositionalLanguage.L Var),
-    forall m: @model _ (TrivialSemantics.SM Var),
+    forall m: @model (TrivialSemantics.MD Var),
       m |= FF --> x.
 Proof.
   intros.
@@ -114,7 +114,7 @@ Qed.
 
 Lemma sound_excluded_middle {Var: Type}:
   forall x: @expr (PropositionalLanguage.L Var),
-    forall m: @model _ (TrivialSemantics.SM Var),
+    forall m: @model (TrivialSemantics.MD Var),
       m |= x || (x --> FF).
 Proof.
   intros.
