PropositionalLogic/Sound_Kripke.v
@@ -13,8 +13,9 @@ Require Import Logic.PropositionalLogic.GodelDummettLogic.
 
 Local Open Scope logic_base.
 Local Open Scope PropositionalLogic.
+Local Open Scope KripkeSemantics.
 
-Lemma sound_modus_ponens {L: Language} {nL: NormalLanguage L} {pL: PropositionalLanguage L} {SM: Semantics L} {pkSM: PreKripkeSemantics L SM} {kiM: KripkeIntuitionisticModel L SM} {kiSM: KripkeIntuitionisticSemantics L SM}:
+Lemma sound_modus_ponens {L: Language} {nL: NormalLanguage L} {pL: PropositionalLanguage L} {MD: Model} {kMD: KripkeModel MD} {kiMD: KripkeIntuitionisticModel MD} {SM: Semantics L MD} {kiSM: KripkeIntuitionisticSemantics L MD SM}:
   forall x y: expr,
     forall M m,
       KRIPKE: M, m |= (x --> y) -> KRIPKE: M, m |= x -> KRIPKE: M, m |= y.
@@ -27,7 +28,7 @@ Proof.
   reflexivity.
 Qed.
 
-Lemma sound_axiom1 {L: Language} {nL: NormalLanguage L} {pL: PropositionalLanguage L} {SM: Semantics L} {pkSM: PreKripkeSemantics L SM} {kiM: KripkeIntuitionisticModel L SM} {kiSM: KripkeIntuitionisticSemantics L SM}:
+Lemma sound_axiom1 {L: Language} {nL: NormalLanguage L} {pL: PropositionalLanguage L} {MD: Model} {kMD: KripkeModel MD} {kiMD: KripkeIntuitionisticModel MD} {SM: Semantics L MD} {kiSM: KripkeIntuitionisticSemantics L MD SM}:
   forall x y: expr,
     forall M m,
       KRIPKE: M, m |= x --> y --> x.
@@ -38,7 +39,7 @@ Proof.
   eapply sat_mono; eauto.
 Qed.
 
-Lemma sound_axiom2 {L: Language} {nL: NormalLanguage L} {pL: PropositionalLanguage L} {SM: Semantics L} {pkSM: PreKripkeSemantics L SM} {kiM: KripkeIntuitionisticModel L SM} {kiSM: KripkeIntuitionisticSemantics L SM}:
+Lemma sound_axiom2 {L: Language} {nL: NormalLanguage L} {pL: PropositionalLanguage L} {MD: Model} {kMD: KripkeModel MD} {kiMD: KripkeIntuitionisticModel MD} {SM: Semantics L MD} {kiSM: KripkeIntuitionisticSemantics L MD SM}:
   forall x y z: expr,
     forall M m,
       KRIPKE: M, m |= (x --> y --> z) --> (x --> y) --> (x --> z).
@@ -61,7 +62,7 @@ Proof.
   auto.
 Qed.
 
-Lemma sound_andp_intros {L: Language} {nL: NormalLanguage L} {pL: PropositionalLanguage L} {SM: Semantics L} {pkSM: PreKripkeSemantics L SM} {kiM: KripkeIntuitionisticModel L SM} {kiSM: KripkeIntuitionisticSemantics L SM}:
+Lemma sound_andp_intros {L: Language} {nL: NormalLanguage L} {pL: PropositionalLanguage L} {MD: Model} {kMD: KripkeModel MD} {kiMD: KripkeIntuitionisticModel MD} {SM: Semantics L MD} {kiSM: KripkeIntuitionisticSemantics L MD SM}:
   forall x y: expr,
     forall M m,
       KRIPKE: M, m |= x --> y --> x && y.
@@ -75,7 +76,7 @@ Proof.
   + auto.
 Qed.
 
-Lemma sound_andp_elim1 {L: Language} {nL: NormalLanguage L} {pL: PropositionalLanguage L} {SM: Semantics L} {pkSM: PreKripkeSemantics L SM} {kiM: KripkeIntuitionisticModel L SM} {kiSM: KripkeIntuitionisticSemantics L SM}:
+Lemma sound_andp_elim1 {L: Language} {nL: NormalLanguage L} {pL: PropositionalLanguage L} {MD: Model} {kMD: KripkeModel MD} {kiMD: KripkeIntuitionisticModel MD} {SM: Semantics L MD} {kiSM: KripkeIntuitionisticSemantics L MD SM}:
   forall x y: expr,
     forall M m,
       KRIPKE: M, m |= x && y --> x.
@@ -86,7 +87,7 @@ Proof.
   tauto.
 Qed.
 
-Lemma sound_andp_elim2 {L: Language} {nL: NormalLanguage L} {pL: PropositionalLanguage L} {SM: Semantics L} {pkSM: PreKripkeSemantics L SM} {kiM: KripkeIntuitionisticModel L SM} {kiSM: KripkeIntuitionisticSemantics L SM}:
+Lemma sound_andp_elim2 {L: Language} {nL: NormalLanguage L} {pL: PropositionalLanguage L} {MD: Model} {kMD: KripkeModel MD} {kiMD: KripkeIntuitionisticModel MD} {SM: Semantics L MD} {kiSM: KripkeIntuitionisticSemantics L MD SM}:
   forall x y: expr,
     forall M m,
       KRIPKE: M, m |= x && y --> y.
@@ -97,7 +98,7 @@ Proof.
   tauto.
 Qed.
 
-Lemma sound_orp_intros1 {L: Language} {nL: NormalLanguage L} {pL: PropositionalLanguage L} {SM: Semantics L} {pkSM: PreKripkeSemantics L SM} {kiM: KripkeIntuitionisticModel L SM} {kiSM: KripkeIntuitionisticSemantics L SM}:
+Lemma sound_orp_intros1 {L: Language} {nL: NormalLanguage L} {pL: PropositionalLanguage L} {MD: Model} {kMD: KripkeModel MD} {kiMD: KripkeIntuitionisticModel MD} {SM: Semantics L MD} {kiSM: KripkeIntuitionisticSemantics L MD SM}:
   forall x y: expr,
     forall M m,
       KRIPKE: M, m |= x --> x || y.
@@ -108,7 +109,7 @@ Proof.
   tauto.
 Qed.
 
-Lemma sound_orp_intros2 {L: Language} {nL: NormalLanguage L} {pL: PropositionalLanguage L} {SM: Semantics L} {pkSM: PreKripkeSemantics L SM} {kiM: KripkeIntuitionisticModel L SM} {kiSM: KripkeIntuitionisticSemantics L SM}:
+Lemma sound_orp_intros2 {L: Language} {nL: NormalLanguage L} {pL: PropositionalLanguage L} {MD: Model} {kMD: KripkeModel MD} {kiMD: KripkeIntuitionisticModel MD} {SM: Semantics L MD} {kiSM: KripkeIntuitionisticSemantics L MD SM}:
   forall x y: expr,
     forall M m,
       KRIPKE: M, m |= y --> x || y.
@@ -119,7 +120,7 @@ Proof.
   tauto.
 Qed.
 
-Lemma sound_orp_elim {L: Language} {nL: NormalLanguage L} {pL: PropositionalLanguage L} {SM: Semantics L} {pkSM: PreKripkeSemantics L SM} {kiM: KripkeIntuitionisticModel L SM} {kiSM: KripkeIntuitionisticSemantics L SM}:
+Lemma sound_orp_elim {L: Language} {nL: NormalLanguage L} {pL: PropositionalLanguage L} {MD: Model} {kMD: KripkeModel MD} {kiMD: KripkeIntuitionisticModel MD} {SM: Semantics L MD} {kiSM: KripkeIntuitionisticSemantics L MD SM}:
   forall x y z: expr,
     forall M m,
       KRIPKE: M, m |= (x --> z) --> (y --> z) --> (x || y --> z).
@@ -138,7 +139,7 @@ Proof.
     apply H2; auto.
 Qed.
 
-Lemma sound_falsep_elim {L: Language} {nL: NormalLanguage L} {pL: PropositionalLanguage L} {SM: Semantics L} {pkSM: PreKripkeSemantics L SM} {kiM: KripkeIntuitionisticModel L SM} {kiSM: KripkeIntuitionisticSemantics L SM}:
+Lemma sound_falsep_elim {L: Language} {nL: NormalLanguage L} {pL: PropositionalLanguage L} {MD: Model} {kMD: KripkeModel MD} {kiMD: KripkeIntuitionisticModel MD} {SM: Semantics L MD} {kiSM: KripkeIntuitionisticSemantics L MD SM}:
   forall x: expr,
     forall M m,
       KRIPKE: M, m |= FF --> x.
@@ -149,10 +150,9 @@ Proof.
   tauto.
 Qed.
 
-Lemma sound_excluded_middle_ident {L: Language} {nL: NormalLanguage L} {pL: PropositionalLanguage L} {SM: Semantics L} {pkSM: PreKripkeSemantics L SM} {kiM: KripkeIntuitionisticModel L SM} {kiSM: KripkeIntuitionisticSemantics L SM}:
+Lemma sound_excluded_middle_ident {L: Language} {nL: NormalLanguage L} {pL: PropositionalLanguage L} {MD: Model} {kMD: KripkeModel MD} {kiMD: KripkeIntuitionisticModel MD} {SM: Semantics L MD} {kiSM: KripkeIntuitionisticSemantics L MD SM}:
   forall x: expr,
-    forall M,
-      (forall m n, @Korder _ _ _ _ _ _ M m n -> m = n) ->
+    forall M {ikiM: IdenticalKripkeIntuitionisticModel MD M},
       (forall m, KRIPKE: M, m |= x || ~~ x).
 Proof.
   intros.
@@ -160,46 +160,49 @@ Proof.
   rewrite sat_orp, sat_impp.
   destruct (Classical_Prop.classic (KRIPKE: M, m |= x)); auto.
   right; intros.
-  apply H in H1; subst n.
+  apply ikiM in H0; subst n.
   tauto.
 Qed.
 
-Lemma sound_impp_choice_no_branch {L: Language} {nL: NormalLanguage L} {pL: PropositionalLanguage L} {SM: Semantics L} {pkSM: PreKripkeSemantics L SM} {kiM: KripkeIntuitionisticModel L SM} {kiSM: KripkeIntuitionisticSemantics L SM}:
+Lemma sound_impp_choice_no_branch {L: Language} {nL: NormalLanguage L} {pL: PropositionalLanguage L} {MD: Model} {kMD: KripkeModel MD} {kiMD: KripkeIntuitionisticModel MD} {SM: Semantics L MD} {kiSM: KripkeIntuitionisticSemantics L MD SM}:
   forall x y: expr,
-    forall M,
-      (forall m1 m2 n, @Korder _ _ _ _ _ _ M m1 n -> @Korder _ _ _ _ _ _ M m2 n -> @Korder _ _ _ _ _ _ M m1 m2 \/ @Korder _ _ _ _ _ _ M m2 m1) ->
+    forall M {nkiM: NoBranchKripkeIntuitionisticModel MD M},
       (forall m, KRIPKE: M, m |= (x --> y) || (y --> x)).
 Proof.
   intros.
   rewrite sat_orp, !sat_impp.
   apply Classical_Prop.NNPP; intro.
-  apply not_or_and in H0; destruct H0.
+  apply not_or_and in H; destruct H.
+  apply not_all_ex_not in H.
   apply not_all_ex_not in H0.
-  apply not_all_ex_not in H1.
-  destruct H0 as [n1 ?], H1 as [n2 ?].
+  destruct H as [n1 ?], H0 as [n2 ?].
+  apply imply_to_and in H.
   apply imply_to_and in H0.
+  destruct H, H0.
   apply imply_to_and in H1.
-  destruct H0, H1.
   apply imply_to_and in H2.
-  apply imply_to_and in H3.
-  destruct H2, H3.
-  specialize (H n1 n2 m H0 H1).
-  destruct H.
-  + pose proof (sat_mono _ _ _ y H).
+  destruct H1, H2.
+  destruct (Korder_no_branch n1 n2 m H H0).
+  + pose proof (sat_mono _ _ _ y H5).
     tauto.
-  + pose proof (sat_mono _ _ _ x H).
+  + pose proof (sat_mono _ _ _ x H5).
     tauto.
 Qed.
 
 Theorem sound_intuitionistic_kripke_all (Var: Type): sound (IntuitionisticPropositionalLogic.G Var) (KripkeSemantics_All.SM Var).
 Proof.
   hnf; intros.
-  pose (KripkeSemantics_All.SM Var) as SM.
-  pose (KripkeSemantics_All.pkSM Var) as pkSM.
-  pose (KripkeSemantics_All.kiSM Var) as kiSM.
+  pose (PropositionalLanguage.L Var) as L.
+  pose (PropositionalLanguage.nL Var: NormalLanguage L) as nL.
+  pose (PropositionalLanguage.pL Var: PropositionalLanguage L) as pL.
+  pose (KripkeSemantics_All.MD Var) as MD.
+  pose (KripkeSemantics_All.kMD Var: KripkeModel MD) as kMD.
+  pose (KripkeSemantics_All.kiMD Var: KripkeIntuitionisticModel MD) as kiMD.
+  pose (KripkeSemantics_All.SM Var: Semantics L MD) as SM.
+  pose (KripkeSemantics_All.kiSM Var: KripkeIntuitionisticSemantics L MD SM) as kiSM.
   intro m.
   destruct m as [M m].
-  change (@Kmodel _ _ pkSM) in M.
+  change Kmodel in M.
   change (Kworlds M) in m.
   change (KRIPKE: M, m |= x).
   induction H.
@@ -219,12 +222,17 @@ Qed.
 Theorem sound_classical_kripke_identical (Var: Type): sound (ClassicalPropositionalLogic.G Var) (KripkeSemantics_Identical.SM Var).
 Proof.
   hnf; intros.
-  pose (KripkeSemantics_Identical.SM Var) as SM.
-  pose (KripkeSemantics_Identical.pkSM Var) as pkSM.
-  pose (KripkeSemantics_Identical.kiSM Var) as kiSM.
+  pose (PropositionalLanguage.L Var) as L.
+  pose (PropositionalLanguage.nL Var: NormalLanguage L) as nL.
+  pose (PropositionalLanguage.pL Var: PropositionalLanguage L) as pL.
+  pose (KripkeSemantics_Identical.MD Var) as MD.
+  pose (KripkeSemantics_Identical.kMD Var: KripkeModel MD) as kMD.
+  pose (KripkeSemantics_Identical.kiMD Var: KripkeIntuitionisticModel MD) as kiMD.
+  pose (KripkeSemantics_Identical.SM Var: Semantics L MD) as SM.
+  pose (KripkeSemantics_Identical.kiSM Var: KripkeIntuitionisticSemantics L MD SM) as kiSM.
   intro m.
   destruct m as [M m].
-  change (@Kmodel _ _ pkSM) in M.
+  change Kmodel in M.
   change (Kworlds M) in m.
   change (KRIPKE: M, m |= x).
   induction H.
@@ -240,18 +248,24 @@ Proof.
   + apply sound_orp_elim.
   + apply sound_falsep_elim.
   + apply sound_excluded_middle_ident.
+    constructor.
     apply (@KripkeSemantics_Identical.frame_ident Var M).
 Qed.
 
 Theorem sound_weak_classical_kripke_no_branch (Var: Type): sound (GodelDummettPropositionalLogic.G Var) (KripkeSemantics_NoBranch.SM Var).
 Proof.
   hnf; intros.
-  pose (KripkeSemantics_NoBranch.SM Var) as SM.
-  pose (KripkeSemantics_NoBranch.pkSM Var) as pkSM.
-  pose (KripkeSemantics_NoBranch.kiSM Var) as kiSM.
+  pose (PropositionalLanguage.L Var) as L.
+  pose (PropositionalLanguage.nL Var: NormalLanguage L) as nL.
+  pose (PropositionalLanguage.pL Var: PropositionalLanguage L) as pL.
+  pose (KripkeSemantics_NoBranch.MD Var) as MD.
+  pose (KripkeSemantics_NoBranch.kMD Var: KripkeModel MD) as kMD.
+  pose (KripkeSemantics_NoBranch.kiMD Var: KripkeIntuitionisticModel MD) as kiMD.
+  pose (KripkeSemantics_NoBranch.SM Var: Semantics L MD) as SM.
+  pose (KripkeSemantics_NoBranch.kiSM Var: KripkeIntuitionisticSemantics L MD SM) as kiSM.
   intro m.
   destruct m as [M m].
-  change (@Kmodel _ _ pkSM) in M.
+  change Kmodel in M.
   change (Kworlds M) in m.
   change (KRIPKE: M, m |= x).
   induction H.
@@ -267,6 +281,7 @@ Proof.
   + apply sound_orp_elim.
   + apply sound_falsep_elim.
   + apply sound_impp_choice_no_branch.
+    constructor.
     apply (@KripkeSemantics_NoBranch.frame_no_branch Var M).
 Qed.
 
