SeparationLogic/DownwardsSemantics.v
@@ -1,27 +1,31 @@
 Require Import Coq.Logic.Classical_Prop.
 Require Import Logic.lib.Coqlib.
 Require Import Logic.MinimunLogic.LogicBase.
-Require Import Logic.MinimunLogic.MinimunLogic.
 Require Import Logic.PropositionalLogic.Syntax.
 Require Import Logic.SeparationLogic.Syntax.
 Require Import Logic.PropositionalLogic.KripkeSemantics.
+Require Import Logic.SeparationLogic.SeparationAlgebra.
 
 Local Open Scope logic_base.
 Local Open Scope PropositionalLogic.
+Local Open Scope KripkeSemantics.
 Local Open Scope SeparationLogic.
 
-Class DownwardsSemantics (L: Language) {nL: NormalLanguage L} {pL: PropositionalLanguage L} {SL: SeparationLanguage L} (SM: Semantics L) {pkSM: PreKripkeSemantics L SM} {kiM: KripkeIntuitionisticModel L SM} {kiSM: KripkeIntuitionisticSemantics L SM} : Type := {
-  join: forall {M: Kmodel}, Kworlds M -> Kworlds M -> Kworlds M -> Prop;
-  join_comm: forall M (m1 m2 m: Kworlds M), join m1 m2 m -> join m2 m1 m;
-  join_assoc: forall M (mx my mz mxy mxyz: Kworlds M), join mx my mxy -> join mxy mz mxyz -> exists myz, join my mz myz /\ join mx myz mxyz;
-  join_Korder: forall M (m n m1 m2: Kworlds M), join m1 m2 m -> Korder n m -> exists n1 n2, join n1 n2 n /\ Korder n1 m1 /\ Korder n2 m2;
-  sat_sepcon: forall M m x y, KRIPKE: M , m |= x * y <-> exists m1 m2, join m1 m2 m /\ KRIPKE: M , m1 |= x /\ KRIPKE: M, m2 |= y;
-  sat_wand: forall M m x y, KRIPKE: M , m |= x -* y <-> forall m0 m1 m2, Korder m0 m -> join m0 m1 m2 -> KRIPKE: M , m1 |= x -> KRIPKE: M, m2 |= y
+Class DownwardsClosedSeparationAlgebra (MD: Model) {kMD: KripkeModel MD} {kiMD: KripkeIntuitionisticModel MD} {SA: SeparationAlgebra MD} (M: Kmodel): Type := {
+  join_Korder_down: forall (m n m1 m2: Kworlds M), join m1 m2 m -> n <= m -> exists n1 n2, join n1 n2 n /\ n1 <= m1 /\ n2 <= m2
 }.
 
-Class UnitaryDownwardsSemantics (L: Language) {nL: NormalLanguage L} {pL: PropositionalLanguage L} {SL: SeparationLanguage L} {uSL: UnitarySeparationLanguage L} (SM: Semantics L) {pkSM: PreKripkeSemantics L SM} {kiM: KripkeIntuitionisticModel L SM} {kiSM: KripkeIntuitionisticSemantics L SM} {dsSM: DownwardsSemantics L SM}: Type := {
-  unit := fun M (m: Kworlds M) => forall n n', join m n n' -> Korder n' n;
-  unit_exists: forall M (n: Kworlds M), exists m, join m n n /\ (forall m', Korder m' m -> unit M m');
-  sat_emp: forall M (m: Kworlds M), KRIPKE: M, m |= emp <-> forall n, Korder n m -> unit M n
+Class DownwardsSemantics (L: Language) {nL: NormalLanguage L} {pL: PropositionalLanguage L} {SL: SeparationLanguage L} (MD: Model) {kMD: KripkeModel MD} {kiMD: KripkeIntuitionisticModel MD} {SA: SeparationAlgebra MD} (SM: Semantics L MD) {kiSM: KripkeIntuitionisticSemantics L MD SM}: Type := {
+  sat_sepcon: forall M m x y, KRIPKE: M , m |= x * y <-> exists m1 m2, join m1 m2 m /\ KRIPKE: M , m1 |= x /\ KRIPKE: M, m2 |= y;
+  sat_wand: forall M m x y, KRIPKE: M , m |= x -* y <-> forall m0 m1 m2, m0 <= m -> join m0 m1 m2 -> KRIPKE: M , m1 |= x -> KRIPKE: M, m2 |= y
+}.
+
+Class DownwardsClosedUnitarySeparationAlgebra (MD: Model) {kMD: KripkeModel MD} {kiMD: KripkeIntuitionisticModel MD} {SA: SeparationAlgebra MD} {USA: UnitarySeparationAlgebra MD} (M: Kmodel): Type := {
+  unit_spec : forall m: Kworlds M, unit m <-> forall n n', join m n n' -> n' <= n;
+  unit_exists: forall n: Kworlds M, exists m, join m n n /\ (forall m', m' <= m -> unit m')
+}.
+
+Class UnitaryDownwardsSemantics (L: Language) {nL: NormalLanguage L} {pL: PropositionalLanguage L} {SL: SeparationLanguage L} {uSL: UnitarySeparationLanguage L} (MD: Model) {kMD: KripkeModel MD} {kiMD: KripkeIntuitionisticModel MD} {SA: SeparationAlgebra MD} {USA: UnitarySeparationAlgebra MD} (SM: Semantics L MD) {kiSM: KripkeIntuitionisticSemantics L MD SM} {dsSM: DownwardsSemantics L MD SM}: Type := {
+  sat_emp: forall M (m: Kworlds M), KRIPKE: M, m |= emp <-> forall n, n <= m -> unit n
 }.
 
