SeparationLogic/UpwardsSemantics.v
@@ -1,22 +1,18 @@
 Require Import Coq.Logic.Classical_Prop.
 Require Import Logic.lib.Coqlib.
 Require Import Logic.MinimunLogic.LogicBase.
-Require Import Logic.MinimunLogic.MinimunLogic.
 Require Import Logic.PropositionalLogic.Syntax.
 Require Import Logic.SeparationLogic.Syntax.
 Require Import Logic.PropositionalLogic.KripkeSemantics.
+Require Import Logic.SeparationLogic.SeparationAlgebra.
 
 Local Open Scope logic_base.
 Local Open Scope PropositionalLogic.
+Local Open Scope KripkeSemantics.
 Local Open Scope SeparationLogic.
 
-Class UpwardsSemantics (L: Language) {nL: NormalLanguage L} {pL: PropositionalLanguage L} {SL: SeparationLanguage L} (SM: Semantics L) {pkSM: PreKripkeSemantics L SM} {kiM: KripkeIntuitionisticModel L SM} {kiSM: KripkeIntuitionisticSemantics L SM} : Type := {
-  join: forall {M: Kmodel}, Kworlds M -> Kworlds M -> Kworlds M -> Prop;
-  join_comm: forall M (m1 m2 m: Kworlds M), join m1 m2 m -> join m2 m1 m;
-  join_assoc: forall M (mx my mz mxy mxyz: Kworlds M), join mx my mxy -> join mxy mz mxyz -> exists myz, join my mz myz /\ join mx myz mxyz;
-  join_Korder: forall M (m1 m2 m n1 n2: Kworlds M), join m1 m2 m -> Korder m1 n1 -> Korder m2 n2 -> exists n, join n1 n2 n /\ Korder m n;
-  sat_sepcon: forall M m x y, KRIPKE: M , m |= x * y <-> exists m0 m1 m2, Korder m m0 /\ join m1 m2 m0 /\ KRIPKE: M , m1 |= x /\ KRIPKE: M, m2 |= y;
-  sat_wand: forall M m x y, KRIPKE: M , m |= x -* y <-> forall m1 m2, join m m1 m2 -> KRIPKE: M , m1 |= x -> KRIPKE: M, m2 |= y
+Class UpwardsClosedSeparationAlgebra (MD: Model) {kMD: KripkeModel MD} {kiMD: KripkeIntuitionisticModel MD} {SA: SeparationAlgebra MD} (M: Kmodel): Type := {
+  join_Korder: forall (m1 m2 m n1 n2: Kworlds M), join m1 m2 m -> m1 <= n1 -> m2 <= n2 -> exists n, join n1 n2 n /\ m <= n
 }.
 
 (* David J. Pym, Peter W. O’Hearn, and Hongseok Yang. Possible worlds and resources: the semantics of BI. *)
@@ -27,9 +23,17 @@ Class UpwardsSemantics (L: Language) {nL: NormalLanguage L} {pL: PropositionalLa
 It is necessary to be this strong, or else sepcon_assoc will be unsound, e.g. the following weaker version causes unsoundness:
   join_Korder: forall M (m1 m2 m n1: Kworlds M), join m1 m2 m -> Korder m1 n1 -> exists n2 n, join n1 n2 n /\ Korder m2 n2 /\ Korder m n;  *)
 
-Class UnitaryUpwardsSemantics (L: Language) {nL: NormalLanguage L} {pL: PropositionalLanguage L} {SL: SeparationLanguage L} {uSL: UnitarySeparationLanguage L} (SM: Semantics L) {pkSM: PreKripkeSemantics L SM} {kiM: KripkeIntuitionisticModel L SM} {kiSM: KripkeIntuitionisticSemantics L SM} {usSM: UpwardsSemantics L SM}: Type := {
-  unit := fun M (m: Kworlds M) => forall n n', join m n n' -> n = n';
-  unit_exists: forall M (n: Kworlds M), exists m, join m n n /\ unit M m;
-  sat_emp: forall M (m: Kworlds M), KRIPKE: M, m |= emp <-> exists n, Korder m n /\ unit M n
+Class UpwardsSemantics (L: Language) {nL: NormalLanguage L} {pL: PropositionalLanguage L} {SL: SeparationLanguage L} (MD: Model) {kMD: KripkeModel MD} {kiMD: KripkeIntuitionisticModel MD} {SA: SeparationAlgebra MD} (SM: Semantics L MD) {kiSM: KripkeIntuitionisticSemantics L MD SM}: Type := {
+  sat_sepcon: forall M m x y, KRIPKE: M , m |= x * y <-> exists m0 m1 m2, m <= m0 /\ join m1 m2 m0 /\ KRIPKE: M , m1 |= x /\ KRIPKE: M, m2 |= y;
+  sat_wand: forall M m x y, KRIPKE: M , m |= x -* y <-> forall m1 m2, join m m1 m2 -> KRIPKE: M , m1 |= x -> KRIPKE: M, m2 |= y
+}.
+
+Class UpwardsClosedUnitarySeparationAlgebra (MD: Model) {kMD: KripkeModel MD} {kiMD: KripkeIntuitionisticModel MD} {SA: SeparationAlgebra MD} {USA: UnitarySeparationAlgebra MD} (M: Kmodel): Type := {
+  unit_spec: forall m: Kworlds M, unit m <-> forall n n', join m n n' -> n = n';
+  unit_exists: forall n: Kworlds M, exists m, join m n n /\ unit m
+}.
+
+Class UnitaryUpwardsSemantics (L: Language) {nL: NormalLanguage L} {pL: PropositionalLanguage L} {SL: SeparationLanguage L} {uSL: UnitarySeparationLanguage L} (MD: Model) {kMD: KripkeModel MD} {kiMD: KripkeIntuitionisticModel MD} {SA: SeparationAlgebra MD} {USA: UnitarySeparationAlgebra MD} (SM: Semantics L MD) {kiSM: KripkeIntuitionisticSemantics L MD SM} {usSM: UpwardsSemantics L MD SM}: Type := {
+  sat_emp: forall M (m: Kworlds M), KRIPKE: M, m |= emp <-> exists n, m <= n /\ unit n
 }.
 
